Proj.thy
@@ -13,21 +13,23 @@ theory Proj
 begin
 
 
-abbreviation fst :: "Term \<Rightarrow> Term" where "fst \<equiv> \<lambda>p. ind\<^sub>\<Sum>(\<lambda>x y. x)(p)"
-abbreviation snd :: "Term \<Rightarrow> Term" where "snd \<equiv> \<lambda>p. ind\<^sub>\<Sum>(\<lambda>x y. y)(p)"
+axiomatization fst :: "Term \<Rightarrow> Term" where fst_def: "fst \<equiv> \<lambda>p. ind\<^sub>\<Sum>(\<lambda>x y. x)(p)"
+axiomatization snd :: "Term \<Rightarrow> Term" where snd_def: "snd \<equiv> \<lambda>p. ind\<^sub>\<Sum>(\<lambda>x y. y)(p)"
 
 text "Typing judgments and computation rules for the dependent and non-dependent projection functions."
 
 
 lemma fst_type:
   assumes "\<Sum>x:A. B(x): U(i)" and "p: \<Sum>x:A. B(x)" shows "fst(p): A"
+unfolding fst_def
 proof
-  show "A: U(i)" using assms(1) by (rule Sum_forms)
+  show "A: U(i)" using assms(1) by (rule Sum_wellform)
 qed (fact assms | assumption)+
 
 
 lemma fst_comp:
   assumes "A: U(i)" and "B: A \<longrightarrow> U(i)" and "a: A" and "b: B(a)" shows "fst(<a,b>) \<equiv> a"
+unfolding fst_def
 proof
   show "\<And>x. x: A \<Longrightarrow> x: A" .
 qed (rule assms)+
@@ -35,25 +37,27 @@ qed (rule assms)+
 
 lemma snd_type:
   assumes "\<Sum>x:A. B(x): U(i)" and "p: \<Sum>x:A. B(x)" shows "snd(p): B(fst p)"
+unfolding snd_def
 proof
   show "\<And>p. p: \<Sum>x:A. B(x) \<Longrightarrow> B(fst p): U(i)"
   proof -
     have "\<And>p. p: \<Sum>x:A. B(x) \<Longrightarrow> fst(p): A" using assms(1) by (rule fst_type)
-    with assms(1) show "\<And>p. p: \<Sum>x:A. B(x) \<Longrightarrow> B(fst p): U(i)" by (rule Sum_forms)
+    with assms(1) show "\<And>p. p: \<Sum>x:A. B(x) \<Longrightarrow> B(fst p): U(i)" by (rule Sum_wellform)
   qed
 
   fix x y
   assume asm: "x: A" "y: B(x)"
   show "y: B(fst <x,y>)"
   proof (subst fst_comp)
-    show "A: U(i)" using assms(1) by (rule Sum_forms)
-    show "\<And>x. x: A \<Longrightarrow> B(x): U(i)" using assms(1) by (rule Sum_forms)
+    show "A: U(i)" using assms(1) by (rule Sum_wellform)
+    show "\<And>x. x: A \<Longrightarrow> B(x): U(i)" using assms(1) by (rule Sum_wellform)
   qed (rule asm)+
 qed (fact assms)
 
 
 lemma snd_comp:
   assumes "A: U(i)" and "B: A \<longrightarrow> U(i)" and "a: A" and "b: B(a)" shows "snd(<a,b>) \<equiv> b"
+unfolding snd_def
 proof
   show "\<And>x y. y: B(x) \<Longrightarrow> y: B(x)" .
   show "a: A" by (fact assms)
@@ -61,6 +65,9 @@ proof
   show *: "B(a): U(i)" using assms(3) by (rule assms(2))
   show "B(a): U(i)" by (fact *)
 qed
+
+
+lemmas Proj_comps [intro] = fst_comp snd_comp
 
 
 end
